src/Bedrock/Group/ScalarMult/LadderStep.v
@@ -20,322 +20,6 @@ Section __.
           {field_representation_ok : FieldRepresentation_ok}.
   Hint Resolve relax_bounds : compiler.
 
-  (*
-  (*Modified from stack_alloc*)
-  Definition felem_alloc : Comp (felem) := fun _ => True.
-   *)
-
-  Definition felem_alloc (v : F M_pos) := v.
-  Arguments felem_alloc : simpl never.
-  
-  Lemma compile_felem_alloc
-        (tr : Semantics.trace)
-        (mem locals : map.rep)
-        (functions : list (string * (list string * list string * cmd)))
-        (e : felem) :
-    let v := (feval e)%F in
-    forall (P : F M_pos -> Type)
-           (pred : P v -> predicate)
-           (k : nlet_eq_k P v) (v_impl k_impl : cmd)
-           (Rin Rout : map.rep -> Prop)
-           (out : felem)
-           (out_var : string),
-      (*
-      (FElem out_ptr out ⋆ Rout) mem ->
-      (FElem e_ptr e ⋆ Rin) mem ->
-       *)
-      Rout mem ->
-      Rin mem ->
-      bounded_by loose_bounds e ->
-      (let v0 := v in
-       forall (out0 : felem) (out_ptr : word.rep) (m : map.rep),
-         feval out0 = v0 ->
-         bounded_by loose_bounds out0 ->
-         (Placeholder out_ptr ⋆ Rout) m ->
-         <{ Trace := tr;
-            Memory := m;
-            Locals := map.put locals out_var out_ptr;
-            Functions := functions }>
-         v_impl
-         <{ fun tr' mem l => tr' = tr /\ (FElem out_ptr out0 ⋆ Rout) mem /\ l = map.put locals out_var out_ptr }>) ->
-      (let v0 := v in
-       forall (out0 : felem) (out_ptr : word.rep) (m : map.rep),
-         feval out0 = v0 ->
-         bounded_by loose_bounds out0 ->
-         (FElem out_ptr out0 ⋆ Rout) m ->
-         <{ Trace := tr;
-            Memory := m;
-            Locals := map.put locals out_var out_ptr;
-            Functions := functions }>
-         k_impl
-         <{fun tr' mem' locals' =>
-             exists m' mStack' : map.rep, Placeholder out_ptr mStack' /\
-                                          map.split mem' m' mStack' /\
-                                          pred (k v0 eq_refl) tr' m' locals' }>) ->
-      <{ Trace := tr;
-         Memory := mem;
-         Locals := locals;
-         Functions := functions }>
-      cmd.stackalloc out_var (@felem_size_in_bytes field_parameters _ field_representaton)
-                     (cmd.seq v_impl k_impl)
-      <{ pred (let/n x as out_var eq:Heq := felem_alloc v in
-               k x Heq) }>.
-  Proof.
-    red.
-    red.
-    cbn.
-    intros.
-    split; eauto using felem_size_in_bytes_mod.
-    change (Memory.anybytes ?p felem_size_in_bytes ?m) with (Placeholder p m).
-    intros ptr mStack mCombined Hany Hsplit.
-    eapply WeakestPrecondition_weaken; cycle 1.
-    - eapply H2; eauto.
-      exists mStack.
-      exists mem.
-      intuition.
-      apply map.split_comm; eauto.
-    - intros tr' mem' locals' [Htr [Hmem Hloc]]; subst.
-      unfold felem_alloc.
-      unfold nlet_eq.
-      eapply H3; eauto.
-  Qed.
-
-  (*
-   Local Ltac prove_field_compilation :=
-    repeat straightline';
-    handle_call;
-    lazymatch goal with
-    | |- sep _ _ _ => ecancel_assumption
-    | _ => idtac
-    end; eauto;
-    sepsimpl; repeat straightline'; subst; eauto.
-   *)
-
-  Definition pred_sep {A} R (pred : A -> predicate) (v : A) tr' mem' locals':=
-    (R * Basics.flip (pred v tr') locals')%sep mem'.
-  
-  Lemma compile_binop_alloc {name} {op: BinOp name}
-        {tr mem locals functions} x y:
-    let v := felem_alloc (bin_model (feval x) (feval y)) in
-    forall {P} {pred: P v -> predicate} {k: nlet_eq_k P v} {k_impl}
-      Rin x_ptr x_var y_ptr y_var out_var,
-
-      (_: spec_of name) functions ->
-      bounded_by bin_xbounds x ->
-      bounded_by bin_ybounds y ->
-
-      (*
-      map.get locals out_var = Some out_ptr ->
-       
-      (FElem out_ptr out * Rout)%sep mem ->
-       *)
-      (*Rout mem -> TODO: is this okay?*)
-      let Rout := (FElem x_ptr x * FElem y_ptr y * Rin)%sep in
-      (FElem x_ptr x * FElem y_ptr y * Rin)%sep mem ->
-      map.get locals x_var = Some x_ptr ->
-      map.get locals y_var = Some y_ptr ->
-
-      out_var <> x_var ->
-      out_var <> y_var ->
-
-      (let v := v in
-       forall out out_ptr m (Heq: feval out = v),
-         bounded_by bin_outbounds out ->
-         sep (FElem out_ptr out) Rout m ->
-         (<{ Trace := tr;
-             Memory := m;
-             Locals := map.put locals out_var out_ptr;
-             Functions := functions }>
-          k_impl
-          <{ pred_sep (Placeholder out_ptr) pred (k v eq_refl) }>)) ->
-      <{ Trace := tr;
-         Memory := mem;
-         Locals := locals;
-         Functions := functions }>
-      
-      cmd.stackalloc out_var (@felem_size_in_bytes field_parameters _ field_representaton)
-                     (cmd.seq
-                        (cmd.call [] name [expr.var out_var; expr.var x_var; expr.var y_var ])
-                        k_impl)
-      <{ pred (nlet_eq [out_var] v k) }>.
-  Proof.
-    repeat straightline'.
-    split; eauto using felem_size_in_bytes_mod.
-    intros out_ptr mStack mCombined Hplace%FElem_from_bytes.
-    destruct Hplace as [out Hout].
-    repeat straightline'.
-    straightline_call.
-    intuition eauto.
-    {
-      exists (FElem out_ptr out * Rin)%sep.
-      assert (((FElem x_ptr x ⋆ FElem y_ptr y ⋆ Rin) * FElem out_ptr out)%sep mCombined).
-      exists mem.
-      exists mStack.
-      intuition.
-      ecancel_assumption.
-    }
-    {
-      exists mStack.
-      exists mem.
-      intuition eauto.
-      apply map.split_comm; eauto.
-    }
-    repeat straightline'.
-    eapply WeakestPrecondition_weaken with (p1 := pred_sep (Memory.anybytes out_ptr felem_size_in_bytes)
-                                                           pred (let/n x as out_var eq:Heq := v in
-                                                                 k x Heq)).
-    {
-      unfold pred_sep.
-      repeat straightline'.
-      destruct H9 as [mStack' [m' [Hmem [HmStack Hm]]]].
-      unfold Basics.flip in Hm.
-      exists m'.
-      exists mStack'.
-      intuition.
-      apply map.split_comm; auto.
-    }
-    eapply H7; repeat straightline'.
-    {
-      unfold v.
-      unfold felem_alloc.
-      eauto.
-    }
-    eauto.
-    {
-      unfold Rout.
-      ecancel_assumption.
-    }
-  Qed.
-
-   Ltac cleanup_op_lemma lem := (* This makes [simple apply] work *)
-    let lm := fresh in
-    let op := match lem with _ _ ?op => op end in
-    let op_hd := term_head op in
-    let simp proj :=
-        (let hd := term_head proj in
-         let reduced := (eval cbv [op_hd hd] in proj) in
-         change proj with reduced in (type of lm)) in
-    pose lem as lm;
-    first [ simp (bin_model (BinOp := op));
-            simp (bin_xbounds (BinOp := op));
-            simp (bin_ybounds (BinOp := op));
-            simp (bin_outbounds (BinOp := op))
-          | simp (un_model (UnOp := op));
-            simp (un_xbounds (UnOp := op));
-            simp (un_outbounds (UnOp := op)) ];
-    let t := type of lm in
-    let t := (eval cbv beta in t) in
-    exact (lm: t).
-  
-  Notation make_bin_alloc_lemma op :=
-    ltac:(cleanup_op_lemma (@compile_binop_alloc _ op)) (only parsing).
-
-  Definition compile_mul := make_bin_alloc_lemma bin_mul.
-  Definition compile_add := make_bin_alloc_lemma bin_add.
-  Definition compile_sub := make_bin_alloc_lemma bin_sub.
-
-  
-   Lemma compile_unop_alloc {name} (op: UnOp name) {tr mem locals functions} x:
-    let v := felem_alloc (un_model (feval x)) in
-    forall {P} {pred: P v -> predicate} {k: nlet_eq_k P v} {k_impl}
-      Rin x_ptr x_var out_var,
-
-      (_: spec_of name) functions ->
-      bounded_by un_xbounds x ->
-
-      
-      let Rout := (FElem x_ptr x * Rin)%sep in
-      (*
-        map.get locals out_var = Some out_ptr ->
-        (FElem out_ptr out * Rout)%sep mem ->
-       *)
-
-      (FElem x_ptr x * Rin)%sep mem ->
-      map.get locals x_var = Some x_ptr ->
-      out_var <> x_var ->
-
-      (let v := v in
-       forall out out_ptr m (Heq : feval out = v),
-         bounded_by un_outbounds out ->
-         sep (FElem out_ptr out) Rout m ->
-         (<{ Trace := tr;
-             Memory := m;
-             Locals := map.put locals out_var out_ptr;
-             Functions := functions }>
-          k_impl
-          <{ pred_sep (Placeholder out_ptr) pred (k v eq_refl)
-
-            (*fun tr' mem' locals' =>
-             exists m' mStack' : map.rep, Placeholder out_ptr mStack' /\
-                                          map.split mem' m' mStack' /\
-                                          pred (k v eq_refl) tr' m' locals' 
-
-             *)}>)) ->
-      <{ Trace := tr;
-         Memory := mem;
-         Locals := locals;
-         Functions := functions }>
-      cmd.stackalloc out_var (@felem_size_in_bytes field_parameters _ field_representaton)
-                     (cmd.seq
-                        (cmd.call [] name [expr.var out_var; expr.var x_var])
-                        k_impl)
-      <{ pred (nlet_eq [out_var] v k) }>.
-   Proof.
-    repeat straightline'.
-    split; eauto using felem_size_in_bytes_mod.
-    intros out_ptr mStack mCombined Hplace%FElem_from_bytes.
-    destruct Hplace as [out Hout].
-    repeat straightline'.
-    straightline_call.
-    intuition eauto.
-    {
-      exists (FElem out_ptr out * Rin)%sep.
-      assert (((FElem x_ptr x ⋆ Rin) * FElem out_ptr out)%sep mCombined).
-      exists mem.
-      exists mStack.
-      intuition.
-      ecancel_assumption.
-    }
-    {
-      exists mStack.
-      exists mem.
-      intuition eauto.
-      apply map.split_comm; eauto.
-    }
-    repeat straightline'.
-    eapply WeakestPrecondition_weaken with (p1 := pred_sep (Memory.anybytes out_ptr felem_size_in_bytes)
-                                                           pred (let/n x as out_var eq:Heq := v in
-                                                                 k x Heq)).
-    {
-      unfold pred_sep.
-      repeat straightline'.
-      destruct H6 as [mStack' [m' [Hmem [HmStack Hm]]]].
-      unfold Basics.flip in Hm.
-      exists m'.
-      exists mStack'.
-      intuition.
-      apply map.split_comm; auto.
-    }
-    eapply H4; repeat straightline'.
-    {
-      unfold v.
-      unfold felem_alloc.
-      eauto.
-    }
-    eauto.
-    {
-      unfold Rout.
-      ecancel_assumption.
-    }
-  Qed.
-
-   Notation make_un_lemma op :=
-     ltac:(cleanup_op_lemma (@compile_unop_alloc _ op)) (only parsing).
-
-   Definition compile_square := make_un_lemma un_square.
-   Definition compile_scmula24 := make_un_lemma un_scmula24.
-   Definition compile_inv := make_un_lemma un_inv.
-
   Section Gallina.
     Local Open Scope F_scope.
 
@@ -343,7 +27,6 @@ Section __.
                (X1: F M_pos) (P1 P2: point) : (point * point) :=
       let '(X2, Z2) := P1 in
       let '(X3, Z3) := P2 in
-      (*TODO: set things up so eq isn't needed *)
       let/n A := felem_alloc (X2+Z2) in
       let/n AA := felem_alloc (A^2) in
       let/n B := felem_alloc (X2-Z2) in
@@ -366,15 +49,13 @@ Section __.
       let/n Z2 := a24*E in
       let/n Z2:= (AA+Z2) in
       let/n Z2 := E*Z2 in
-      (* ((X4, Z4), (X5, Z5)) *)
       ((X2, Z2), (X3, Z3)).
   End Gallina.
 
   Instance spec_of_ladderstep : spec_of "ladderstep" :=
     fnspec! "ladderstep"
-          (pX1 pX2 pZ2 pX3 pZ3
-               (*pA pAA pB pBB pE pC pD pDA pCB*) : Semantics.word)
-          / (X1 X2 Z2 X3 Z3 (*A AA B BB E C D DA CB*) : felem) R,
+          (pX1 pX2 pZ2 pX3 pZ3 : Semantics.word)
+          / (X1 X2 Z2 X3 Z3 : felem) R,
     { requires tr mem :=
         bounded_by tight_bounds X1
         /\ bounded_by tight_bounds X2
@@ -383,16 +64,10 @@ Section __.
         /\ bounded_by tight_bounds Z3
         /\ (FElem pX1 X1
             * FElem pX2 X2 * FElem pZ2 Z2
-            * FElem pX3 X3 * FElem pZ3 Z3
-            (** FElem pA A * FElem pAA AA
-             * FElem pB B * FElem pBB BB
-             * FElem pE E * FElem pC C
-             * FElem pD D * FElem pDA DA
-             * FElem pCB CB*) * R)%sep mem;
+            * FElem pX3 X3 * FElem pZ3 Z3 * R)%sep mem;
       ensures tr' mem' :=
         tr = tr'
         /\ exists X4 Z4 X5 Z5 (* output values *)
-                  (*A' AA' B' BB' E' C' D' DA' CB' (* new intermediates *)*)
                   : felem,
           (ladderstep_gallina
              (feval X1) (feval X2, feval Z2)
@@ -403,11 +78,7 @@ Section __.
           /\ bounded_by tight_bounds X5
           /\ bounded_by tight_bounds Z5
           /\ (FElem pX1 X1 * FElem pX2 X4 * FElem pZ2 Z4
-              * FElem pX3 X5 * FElem pZ3 Z5
-              (** FElem pA A' * FElem pAA AA'
-               * FElem pB B' * FElem pBB BB'
-               * FElem pE E' * FElem pC C' * FElem pD D'
-               * FElem pDA DA' * FElem pCB CB'*) * R)%sep mem'}.
+              * FElem pX3 X5 * FElem pZ3 Z5 * R)%sep mem'}.
 
   Lemma compile_ladderstep : forall {tr mem locals functions}
         (x1 x2 z2 x3 z3 : F M_pos),
@@ -415,12 +86,7 @@ Section __.
     forall {P} {pred: P v -> predicate} {k: nlet_eq_k P v} {k_impl}
            Rout
            X1 X1_ptr X1_var X2 X2_ptr X2_var Z2 Z2_ptr Z2_var
-           X3 X3_ptr X3_var Z3 Z3_ptr Z3_var
-    (* A A_ptr A_var AA AA_ptr AA_var
-           B B_ptr B_var BB BB_ptr BB_var
-           E E_ptr E_var C C_ptr C_var
-           D D_ptr D_var DA DA_ptr DA_var
-           CB CB_ptr CB_var*),
+           X3 X3_ptr X3_var Z3 Z3_ptr Z3_var,
 
       spec_of_ladderstep functions ->
 
@@ -436,31 +102,16 @@ Section __.
       bounded_by tight_bounds Z3 ->
       (FElem X1_ptr X1
        * FElem X2_ptr X2 * FElem Z2_ptr Z2
-       * FElem X3_ptr X3 * FElem Z3_ptr Z3
-      (* * FElem A_ptr A * FElem AA_ptr AA
-       * FElem B_ptr B * FElem BB_ptr BB
-       * FElem E_ptr E * FElem C_ptr C
-       * FElem D_ptr D * FElem DA_ptr DA
-       * FElem CB_ptr CB *) * Rout)%sep mem ->
+       * FElem X3_ptr X3 * FElem Z3_ptr Z3 * Rout)%sep mem ->
 
         map.get locals X1_var = Some X1_ptr ->
         map.get locals X2_var = Some X2_ptr ->
         map.get locals Z2_var = Some Z2_ptr ->
         map.get locals X3_var = Some X3_ptr ->
         map.get locals Z3_var = Some Z3_ptr ->
-        (*map.get locals A_var = Some A_ptr ->
-        map.get locals AA_var = Some AA_ptr ->
-        map.get locals B_var = Some B_ptr ->
-        map.get locals BB_var = Some BB_ptr ->
-        map.get locals E_var = Some E_ptr ->
-        map.get locals C_var = Some C_ptr ->
-        map.get locals D_var = Some D_ptr ->
-        map.get locals DA_var = Some DA_ptr ->
-        map.get locals CB_var = Some CB_ptr ->*)
 
         (let v := v in
          forall (X4 Z4 X5 Z5 (* output values *)
-                    (*A' AA' B' BB' E' C' D' DA' CB' (* new intermediates *)*)
                  : felem) m
                 (Heq : ladderstep_gallina
                          (feval X1) (feval X2, feval Z2)
@@ -471,11 +122,7 @@ Section __.
           bounded_by tight_bounds X5 ->
           bounded_by tight_bounds Z5 ->
           (FElem X1_ptr X1 * FElem X2_ptr X4 * FElem Z2_ptr Z4
-           * FElem X3_ptr X5 * FElem Z3_ptr Z5
-           (* * FElem A_ptr A' * FElem AA_ptr AA'
-           * FElem B_ptr B' * FElem BB_ptr BB'
-           * FElem E_ptr E' * FElem C_ptr C' * FElem D_ptr D'
-           * FElem DA_ptr DA' * FElem CB_ptr CB' *) * Rout)%sep m ->
+           * FElem X3_ptr X5 * FElem Z3_ptr Z5 * Rout)%sep m ->
            (<{ Trace := tr;
                Memory := m;
                Locals := locals;
@@ -491,11 +138,7 @@ Section __.
           (cmd.call [] "ladderstep"
                     [ expr.var X1_var; expr.var X2_var;
                         expr.var Z2_var; expr.var X3_var;
-                          expr.var Z3_var (*; expr.var A_var;
-                            expr.var AA_var; expr.var B_var;
-                              expr.var BB_var; expr.var E_var;
-                                expr.var C_var; expr.var D_var;
-                                  expr.var DA_var; expr.var CB_var *)])
+                          expr.var Z3_var])
           k_impl
         <{ pred (nlet_eq
                    [X1_var; X2_var; Z2_var; X3_var; Z3_var]
@@ -509,24 +152,6 @@ Section __.
         end.
     Qed.
 
-  (*TODO: move, along with allocating lemma *)
-  Ltac field_compile_step :=
-  (first
-   [ simple eapply compile_scmula24
-   | simple eapply compile_mul
-   | simple eapply compile_add
-   | simple eapply compile_sub
-   | simple eapply compile_square
-   | simple eapply compile_inv
-   | simple eapply Compilation.compile_scmula24
-   | simple eapply Compilation.compile_mul
-   | simple eapply Compilation.compile_add
-   | simple eapply Compilation.compile_sub
-   | simple eapply Compilation.compile_square
-   | simple eapply Compilation.compile_inv ]); lazymatch goal with
-                                   | |- feval _ = _ => try eassumption; try reflexivity
-                                   | |- _ => idtac
-                                   end.
   
   Ltac ladderstep_compile_custom :=
     simple apply compile_nlet_as_nlet_eq;
@@ -539,39 +164,9 @@ Section __.
            end.
 
   Ltac compile_custom ::= ladderstep_compile_custom.
-  
-Definition
-  ladderstep_body' :=
-  noskips
-  (cmd.seq (cmd.call [] add [expr.var "X2"; expr.var "Z2"; expr.var "A"])
-     (cmd.seq (cmd.call [] square [expr.var "A"; expr.var "AA"])
-        (cmd.seq (cmd.call [] sub [expr.var "X2"; expr.var "Z2"; expr.var "B"])
-           (cmd.seq (cmd.call [] square [expr.var "B"; expr.var "BB"])
-              (cmd.seq (cmd.call [] sub [expr.var "AA"; expr.var "BB"; expr.var "E"])
-                 (cmd.seq (cmd.call [] add [expr.var "X3"; expr.var "Z3"; expr.var "C"])
-                    (cmd.seq (cmd.call [] sub [expr.var "X3"; expr.var "Z3"; expr.var "D"])
-                       (cmd.seq (cmd.call [] mul [expr.var "D"; expr.var "A"; expr.var "DA"])
-                          (cmd.seq (cmd.call [] mul [expr.var "C"; expr.var "B"; expr.var "CB"])
-                             (cmd.seq (cmd.call [] add [expr.var "DA"; expr.var "CB"; expr.var "X3"])
-                                (cmd.seq (cmd.call [] square [expr.var "X3"; expr.var "X3"])
-                                   (cmd.seq (cmd.call [] sub [expr.var "DA"; expr.var "CB"; expr.var "Z3"])
-                                      (cmd.seq (cmd.call [] square [expr.var "Z3"; expr.var "Z3"])
-                                         (cmd.seq (cmd.call [] mul [expr.var "X1"; expr.var "Z3"; expr.var "Z3"])
-                                            (cmd.seq
-                                               (cmd.call [] mul [expr.var "AA"; expr.var "BB"; expr.var "X2"])
-                                               (cmd.seq (cmd.call [] scmula24 [expr.var "E"; expr.var "Z2"])
-                                                  (cmd.seq
-                                                     (cmd.call [] add
-                                                        [expr.var "AA"; expr.var "Z2"; expr.var "Z2"])
-                                                     (cmd.seq
-                                                        (cmd.call [] mul
-                                                           [expr.var "E"; expr.var "Z2"; expr.var "Z2"])
-                                                        (fold_right
-                                                           (fun (v : string) (c : cmd) => cmd.seq (cmd.unset v) c)
-                                                           cmd.skip []))))))))))))))))))).
 
-Axiom TODO : False.
-Derive ladderstep_body SuchThat
+  
+  Derive ladderstep_body SuchThat
          (let args := ["X1"; "X2"; "Z2"; "X3"; "Z3"] in
           ltac:(
             let proc := constr:(("ladderstep",
@@ -582,95 +177,9 @@ Derive ladderstep_body SuchThat
             exact (__rupicola_program_marker ladderstep_gallina -> goal)))
          As ladderstep_correct.
 Proof.
-  (*
-  unfold ladderstep_body.
-  instantiate (1:=
-                  noskips
-                       (cmd.stackalloc "A" felem_size_in_bytes
-                          (cmd.seq (cmd.call [] add [expr.var "A"; expr.var "X2"; expr.var "Z2"])
-                             (cmd.stackalloc "AA" felem_size_in_bytes
-                                (cmd.seq (cmd.call [] square [expr.var "AA"; expr.var "A"])
-                                   (cmd.stackalloc "B" felem_size_in_bytes
-                                      (cmd.seq (cmd.call [] sub [expr.var "B"; expr.var "X2"; expr.var "Z2"])
-                                         (cmd.stackalloc "BB" felem_size_in_bytes
-                                            (cmd.seq (cmd.call [] square [expr.var "BB"; expr.var "B"])
-                                               (cmd.stackalloc "E" felem_size_in_bytes
-                                                  (cmd.seq
-                                                     (cmd.call [] sub [expr.var "E"; expr.var "AA"; expr.var "BB"])
-                                                     (cmd.stackalloc "C" felem_size_in_bytes
-                                                        (cmd.seq
-                                                           (cmd.call [] add
-                                                              [expr.var "C"; expr.var "X3"; expr.var "Z3"])
-                                                           (cmd.stackalloc "D" felem_size_in_bytes
-                                                              (cmd.seq
-                                                                 (cmd.call [] sub
-                                                                    [expr.var "D"; expr.var "X3"; expr.var "Z3"])
-                                                                 (cmd.stackalloc "DA" felem_size_in_bytes
-                                                                    (cmd.seq
-                                                                       (cmd.call [] mul
-                                                                          [expr.var "DA"; 
-                                                                          expr.var "D"; 
-                                                                          expr.var "A"])
-                                                                       (cmd.stackalloc "CB" felem_size_in_bytes
-                                                                          (cmd.seq
-                                                                             (cmd.call [] mul
-                                                                                [expr.var "CB"; 
-                                                                                expr.var "C"; 
-                                                                                expr.var "B"])
-                                                                             (cmd.seq
-                                                                                (cmd.call [] add
-                                                                                   [expr.var "X3"; 
-                                                                                   expr.var "DA"; 
-                                                                                   expr.var "CB"])
-                                                                                (cmd.seq
-                                                                                   (cmd.call [] square
-                                                                                     [
-                                                                                     expr.var "X3"; 
-                                                                                     expr.var "X3"])
-                                                                                   (cmd.seq
-                                                                                     (cmd.call [] sub
-                                                                                     [
-                                                                                     expr.var "Z3"; 
-                                                                                     expr.var "DA"; 
-                                                                                     expr.var "CB"]) cmd.skip)))))))))))))))))))))).
-  destruct TODO.
-Qed.*)
 
   compile_setup.
-  do 16 compile_step.
-  (* 3 s*)
-  (*
-  simple apply compile_nlet_as_nlet_eq.
-  field_compile_step.
-  Set Printing Depth 100.
-  9:instantiate(1:= cmd.skip).
-  7:instantiate(2:= "DA").
-  8:instantiate(2:= "CB").
-  all: destruct TODO.
-  
-  destruct TODO.
-Time Qed.
-    Time
-    1-8:repeat compile_step.
-    eauto with compiler;
-    (* rewrite results in terms of feval to match lemmas *)
-    repeat lazymatch goal with
-           | H : feval _ = ?x |- context [?x] =>
-             is_var x; rewrite <-H
-           end.
-  compile_custom.
-*)
-  compile_step.
-  (* 10 s*)
-  compile_step.
-  (*26s *)
-  compile_step.
-  (*96s *)
   repeat compile_step.
- 
-  (*instantiate(1:= cmd.skip).
-  destruct TODO.
-Time Qed. *)
   {
     unfold pred_sep; simpl.
     unfold Basics.flip; simpl.
